update some proofs for new spec

proof/correctness/Repr2.ec
@@ -1,17 +1,64 @@
 pragma Goals : printall.
 
-require import AllCore List.
+require import AllCore List IntDiv.
 
 from Jasmin require import JModel.
 
 (*****) import StdBigop.Bigint.
 
-require import Params WOTS.
+require import Params Types WOTS XMSS_Params XMSS_MT_Types.
 
-require import Array2144.
+require import Array64 Array68 Array132 Array136 Array2144.
+
+require import BitEncoding.
+(*---*) import BitChunking.
 
 (* Encode : impl -> spec *)
 (* Decode : spec -> impl *)
+
+(** -------------------------------------------------------------------------------------------- **)
+
+op W32toBytes (x : W32.t) : W8.t list = map W8.bits2w (chunk W8.size (W32.w2bits x)).
+
+lemma size_W32toBytes (x : W32.t) :
+    size (W32toBytes x) = 4
+        by rewrite /W32toBytes size_map size_chunk // size_w2bits. 
+
+lemma W32toBytes_zero_nth (i : int) :
+    0 <= i < 4 => nth witness (W32toBytes W32.zero) i = W8.zero.
+proof.
+move => H.
+rewrite /W32toBytes.
+rewrite (nth_map witness).
+  + by rewrite size_chunk.
+print w2bits. 
+have ->: w2bits W32.zero = nseq 32 false.
+  + apply (eq_from_nth false); [ by rewrite size_w2bits size_nseq |].
+    rewrite size_w2bits => j?.
+    rewrite get_w2bits nth_nseq //=.
+have ->: chunk 8 (nseq 32 false) = nseq 4 (nseq 8 false).
+  + apply (eq_from_nth witness); [by rewrite size_chunk //= !size_nseq /# |].
+    rewrite size_chunk //= size_nseq (: 32 %/ 8 = 4) 1:/# => j?.
+    rewrite nth_nseq 1:/#.
+    rewrite /chunk nth_mkseq; [by rewrite size_nseq (: 32 %/ 8 = 4) 1:/# |].
+    auto => />. 
+    apply (eq_from_nth witness).
+      * rewrite size_take //= size_drop 1:/# !size_nseq. 
+        rewrite (: (max 0 32) = 32) 1:/# (: max 0 (32 - 8 * j) = (32 - 8 *j)) 1:/# /#. 
+    rewrite size_take //= size_drop 1:/# !size_nseq.      
+    rewrite (: (max 0 32) = 32) 1:/# (: max 0 (32 - 8 * j) = (32 - 8 *j)) 1:/#.
+    move => i0?.
+    rewrite nth_nseq 1:/# nth_take //= 1:/# nth_drop 1,2:/# nth_nseq 1:/# //.
+rewrite nth_nseq //.
+rewrite /W8.zero.
+congr. 
+apply (eq_from_nth false).
+  + rewrite size_nseq /int2bs size_mkseq //=.
+rewrite size_nseq (: max 0 8 = 8) 1:/# => j?.  
+rewrite nth_nseq //= /int2bs nth_mkseq //=.
+qed.
+
+(** -------------------------------------------------------------------------------------------- **)
 
 op nbytes_flatten (x : nbytes list) : W8.t list =
   flatten (map (NBytes.val) x).
@@ -41,3 +88,19 @@ lemma wots_sk_size (sk : wots_sk) : size (val sk) = len by smt(LenNBytes.valP).
 lemma wotS_sk_ssize (sk : wots_sk) :
     forall (t : nbytes), t \in val sk => size (val t) = n
       by smt(NBytes.valP).
+
+(** -------------------------------------------------------------------------------------------- **)
+
+op DecodePk (x : xmss_pk) : W8.t Array68.t = 
+  Array68.of_list witness (W32toBytes impl_oid ++ val x.`pk_root ++ val x.`pk_pub_seed).
+
+op DecodePkNoOID (x : xmss_pk) : W8.t Array64.t = 
+  Array64.of_list witness (val x.`pk_root ++ val x.`pk_pub_seed).
+
+op DecodeSk (x : xmss_sk) : W8.t Array136.t = 
+  Array136.of_list witness (W32toBytes impl_oid ++ W32toBytes x.`idx ++ val x.`sk_seed ++ 
+                            val x.`sk_prf ++ val x.`sk_root ++ val x.`pub_seed_sk).
+
+op DecodeSkNoOID (x : xmss_sk) : W8.t Array132.t = 
+  Array132.of_list witness (W32toBytes x.`idx ++ val x.`sk_seed ++ val x.`sk_prf ++ val x.`sk_root ++ val  x.`pub_seed_sk).
+
