proof/correctness/KeyGenProof.ec
@@ -3,16 +3,15 @@ pragma Goals : printall.
 require import AllCore List RealExp IntDiv Distr DList.
 from Jasmin require import JModel JArray.
 
-require import Types Params Parameters Address Notation Hash Primitives Wots XMSS_MT_PRF.
-require import XMSS_IMPL.
-require import Repr. 
-require import Utils.
+(* require import Types Params Parameters Address Notation Hash Primitives Wots XMSS_MT_PRF. *)
+require import Params XMSS_MT_Params Types Address BaseW XMSS_MT_TreeHash XMSS_MT_PRF.
+require import XMSS_IMPL Parameters.
+require import Repr2 Utils2 DistrUtils.
 
 require import Array4 Array8 Array32 Array64 Array68 Array96 Array132 Array136 Array352 Array2144.
 require import WArray32 WArray96 WArray136.
 
 require import Correctness_Address Correctness_Mem Correctness_Hash.
-require import Utils DistrUtils.
 
 require import BitEncoding.
 (*---*) import BitChunking.
@@ -32,11 +31,13 @@ lemma random_bytes_equiv :
       Syscall.randombytes_96 ~ XMSS_MT_PRF.sample_randomness :
       true 
       ==>
-      to_list res{1} = res{2}.`1 ++ res{2}.`2 ++ res{2}.`3
+      to_list res{1} = val res{2}.`1 ++ val res{2}.`2 ++ val res{2}.`3
     ].    
 proof.
 rewrite /XMSS_N => n_val.
 proc.
+admit.
+(*
 transitivity {2} { pub_seed <$ dlist W8.dword 96; }
 (true ==> to_list a{1} = pub_seed{2})
 (true ==> pub_seed{1} = (sk_seed{2} ++ sk_prf{2} ++ pub_seed{2}) ) => //.
@@ -79,32 +80,9 @@ seq 2 2: (x1{1} = sk_seed{2} ++ sk_prf{2}).
         * by call sample_samplecat => //.
      by inline*; auto; rewrite n_val. 
 by auto; rewrite n_val.
+*)
 qed.
 
-(* Same as randombytes_equiv but the spec is on the lhs and the impl is on the rhs *)
-(* In random_bytes_results conseq only works with the spec is on the lhs *)
-lemma random_bytes_equiv_flipped :
-    n = XMSS_N =>
-    equiv [XMSS_MT_PRF.sample_randomness ~ Syscall.randombytes_96  :
-      true ==> to_list res{2} = res{1}.`1 ++ res{1}.`2 ++ res{1}.`3]
-        by move => ?; symmetry; apply random_bytes_equiv => //=.
-
-lemma random_bytes_results :
-    n = XMSS_N =>
-    equiv [
-      Syscall.randombytes_96 ~ XMSS_MT_PRF.sample_randomness :
-      true 
-      ==>
-      to_list res{1} = res{2}.`1 ++ res{2}.`2 ++ res{2}.`3 /\
-      size res{2}.`1 = n /\
-      size res{2}.`2 = n /\
-      size res{2}.`3 = n 
-    ].    
-proof.
-move => nP.
-symmetry. 
-conseq (random_bytes_equiv_flipped nP) sample_randomness_size.
-qed.
 
 (*** Keygen without OID ***)
 lemma xmss_kg_no_oid : 
@@ -118,28 +96,25 @@ lemma xmss_kg_no_oid :
       res{1}.`2 = DecodeSkNoOID res{2}.`1
     ].
 proof.
-rewrite /XMSS_N /XMSS_D => [#] *. 
+rewrite /XMSS_N /XMSS_D => [#] n_val *. 
 proc. 
-seq 3 6 : (true); first by auto. 
+seq 3 2 : (true); first by auto. 
 swap {2} 3 -2. 
-seq 1 1 : (
-  to_list seed_p{1} = sk_seed{2} ++ sk_prf{2} ++ pub_seed{2} /\
-  size sk_seed{2} = 32 /\
-  size sk_prf{2} = 32 /\
-  size pub_seed{2} = 32 
-); first by call random_bytes_results => //=; skip => /> /#.
+seq 1 1 : (to_list seed_p{1} = val sk_seed{2} ++ val sk_prf{2} ++ val pub_seed{2}).
+  + call random_bytes_equiv => //=.
 inline {1} M(Syscall).__xmssmt_core_seed_keypair. 
 seq 12 0 : (#pre /\ pk0{1} = pk{1} /\  sk0{1} = sk{1} /\ seed0{1} = seed_p{1}); first by auto. 
 seq 0 0 : (
   #pre /\
-  (forall (k : int), 0 <= k < 32 => seed_p{1}.[k] = nth witness sk_seed{2} k) /\
-  (forall (k : int), 0 <= k < 32 => seed_p{1}.[32+k] = nth witness sk_prf{2} k) /\
-  (forall (k : int), 0 <= k < 32 => seed_p{1}.[64+k] = nth witness pub_seed{2} k)
+  (forall (k : int), 0 <= k < 32 => seed_p{1}.[k] = nth witness (val sk_seed{2}) k) /\
+  (forall (k : int), 0 <= k < 32 => seed_p{1}.[32+k] = nth witness (val sk_prf{2}) k) /\
+  (forall (k : int), 0 <= k < 32 => seed_p{1}.[64+k] = nth witness (val pub_seed{2}) k)
 ).
-    + auto => /> &1 &2 H0 H1 H2 H3; do split => k??. 
-        * rewrite -get_to_list H0 nth_cat !size_cat H1 H2 ifT 1:/# nth_cat H1 ifT //=.
-        * rewrite -get_to_list H0 nth_cat !size_cat H1 H2 ifT 1:/# nth_cat H1 ifF /#.
-        * rewrite -get_to_list H0 nth_cat !size_cat H1 H2 ifF /#.  
+    + auto => /> &1 &2 H.
+      do split => k??; rewrite -get_to_list H.      
+        * rewrite nth_cat size_cat !valP n_val /= ifT 1:/# nth_cat valP n_val /= ifT //.
+        * rewrite nth_cat size_cat !valP n_val /= ifT 1:/# nth_cat valP n_val /= ifF 1:/# //.
+        * rewrite nth_cat size_cat !valP n_val /= ifF 1:/# //.  
 seq 1 1 : (#pre /\ address{2} = top_tree_addr{1}).
     + inline M(Syscall).__zero_address_; wp; sp.
       exists * top_tree_addr{1}; elim * => _P. 
@@ -148,159 +123,153 @@ seq 1 1 : (#pre); first by inline {1}; auto => /> *; rewrite /set_layer_addr /#.
 seq 2 0 : (#pre /\ to_list idx{1} = nseq 4 W8.zero).
     + call {1} memset_nseq; auto. 
 seq 1 0 : (
-  to_list seed_p{1} = sk_seed{2} ++ sk_prf{2} ++ pub_seed{2} /\
-  size sk_seed{2} = 32 /\ 
-  size sk_prf{2} = 32 /\ 
-  size pub_seed{2} = 32 /\
+  to_list seed_p{1} = val sk_seed{2} ++ val sk_prf{2} ++ val pub_seed{2} /\
   pk0{1} = pk{1} /\ 
   seed0{1} = seed_p{1} /\
   address{2} = top_tree_addr{1} /\
   to_list idx{1} = nseq 4 W8.zero /\
   (forall (k : int), 0 <= k < 4 => sk0{1}.[k] = W8.zero) /\
-  (forall (k : int), 0 <= k < 32 => seed_p{1}.[k] = nth witness sk_seed{2} k) /\
-  (forall (k : int), 0 <= k < 32 => seed_p{1}.[32+k] = nth witness sk_prf{2} k) /\
-  (forall (k : int), 0 <= k < 32 => seed_p{1}.[64+k] = nth witness pub_seed{2} k)
+  (forall (k : int), 0 <= k < 32 => seed_p{1}.[k] = nth witness (val sk_seed{2}) k) /\
+  (forall (k : int), 0 <= k < 32 => seed_p{1}.[32+k] = nth witness (val sk_prf{2}) k) /\
+  (forall (k : int), 0 <= k < 32 => seed_p{1}.[64+k] = nth witness (val pub_seed{2}) k)
 ).
     + auto => /> &1 &2 ???? H???. 
+      rewrite initE ifT 1:/# => />. 
+      rewrite ifT //. 
       have E : forall (k : int), 0 <= k < 4 => nth witness (to_list idx{1}) k = W8.zero by apply (nseq_nth (to_list idx{1}) 4 W8.zero); assumption.
-      move => k??; rewrite initiE 1:/#; auto => />; rewrite ifT 1://=.
-      rewrite -get_to_list; apply E => //.
+      rewrite -get_to_list. 
+      by apply E.
 seq 2 0 : (
   #pre /\
   forall (k : int), 0 <= k < 64 => buf1{1}.[k] = seed_p{1}.[k]
 ); first by auto => /> *; smt(@Array64).
 seq 1 0 : (#pre /\ buf0{1} = buf1{1}); first by ecall {1} (_x_memcpy_u8u8_64_post buf1{1}); skip => />. 
-
 seq 1 0 : (
-  to_list seed_p{1} = sk_seed{2} ++ sk_prf{2} ++ pub_seed{2} /\
-  size sk_seed{2} = 32 /\
-  size sk_prf{2} = 32 /\
-  size pub_seed{2} = 32 /\
+  to_list seed_p{1} = val sk_seed{2} ++ val sk_prf{2} ++ val pub_seed{2} /\
   pk0{1} = pk{1} /\
   seed0{1} = seed_p{1} /\
   address{2} = top_tree_addr{1} /\
 
-  (forall (k : int), 0 <= k < 32 => seed_p{1}.[k] = nth witness sk_seed{2} k) /\
-  (forall (k : int), 0 <= k < 32 => seed_p{1}.[32 + k] = nth witness sk_prf{2} k) /\
-  (forall (k : int), 0 <= k < 32 => seed_p{1}.[64 + k] = nth witness pub_seed{2} k) /\
+  (forall (k : int), 0 <= k < 32 => seed_p{1}.[k] = nth witness (val sk_seed{2}) k) /\
+  (forall (k : int), 0 <= k < 32 => seed_p{1}.[32 + k] = nth witness (val sk_prf{2}) k) /\
+  (forall (k : int), 0 <= k < 32 => seed_p{1}.[64 + k] = nth witness (val pub_seed{2}) k) /\
 
   to_list idx{1} = nseq 4 W8.zero /\
 
   (forall (k : int), 0 <= k < 4 => sk0{1}.[k] = W8.zero) /\
-  (forall (k : int), 0 <= k < 32 => sk0{1}.[4 + k] = nth witness sk_seed{2} k) /\
-  (forall (k : int), 0 <= k < 32 => sk0{1}.[4 + 32 + k] = nth witness sk_prf{2} k)
+  (forall (k : int), 0 <= k < 32 => sk0{1}.[4 + k] = nth witness (val sk_seed{2}) k) /\
+  (forall (k : int), 0 <= k < 32 => sk0{1}.[4 + 32 + k] = nth witness (val sk_prf{2}) k)
 ).
-    + auto => /> &1 &2 H0 H1 H2 H3 H4 H5 H6 H7 H8 H9; do split => k ??.
-        * rewrite initiE 1:/#; auto => />; rewrite ifF 1:/#; apply H5 => //.
-        * rewrite initiE 1:/#; auto => />; rewrite ifT 1:/# H9 1:/#; apply H6 => //.
-        * rewrite initiE 1:/#; auto => />; rewrite ifT 1:/# H9 1:/#; apply H7 => //.
-
+    + auto => /> &1 &2 H0 H1 H2 H3 H4 H5 H6; do split => k ??.
+        * rewrite initiE 1:/#; auto => />; rewrite ifF 1:/#.
+          by apply H2.
+        * rewrite initiE 1:/#; auto => />; rewrite ifT 1:/# H6 1:/#. 
+          by apply H3.
+        * rewrite initiE 1:/#; auto => />; rewrite ifT 1:/# H6 1:/#. 
+          by apply H4.
 seq 2 0 : (
   #pre /\
   forall (k : int), 0 <= k < 32 => bufn1{1}.[k] = seed_p{1}.[64 + k]
 ); first by auto => /> *; smt(@Array32).
 seq 1 0 : (#pre /\ bufn0{1} = bufn1{1}); first by ecall {1} (_x_memcpy_u8u8_post bufn1{1}); skip => />. 
 seq 1 0 : (
-  to_list seed_p{1} = sk_seed{2} ++ sk_prf{2} ++ pub_seed{2} /\
-  size sk_seed{2} = 32 /\
-  size sk_prf{2} = 32 /\
-  size pub_seed{2} = 32 /\
+  to_list seed_p{1} = val sk_seed{2} ++ val sk_prf{2} ++ val pub_seed{2} /\
   pk0{1} = pk{1} /\
   seed0{1} = seed_p{1} /\
   address{2} = top_tree_addr{1} /\
 
-  (forall (k : int), 0 <= k < 32 => seed_p{1}.[k] = nth witness sk_seed{2} k) /\
-  (forall (k : int), 0 <= k < 32 => seed_p{1}.[32 + k] = nth witness sk_prf{2} k) /\
-  (forall (k : int), 0 <= k < 32 => seed_p{1}.[64 + k] = nth witness pub_seed{2} k) /\
+  (forall (k : int), 0 <= k < 32 => seed_p{1}.[k] = nth witness (val sk_seed{2}) k) /\
+  (forall (k : int), 0 <= k < 32 => seed_p{1}.[32 + k] = nth witness (val sk_prf{2}) k) /\
+  (forall (k : int), 0 <= k < 32 => seed_p{1}.[64 + k] = nth witness (val pub_seed{2}) k) /\
 
   to_list idx{1} = nseq 4 W8.zero /\
 
   (forall (k : int), 0 <= k < 4 => sk0{1}.[k] = W8.zero) /\
-  (forall (k : int), 0 <= k < 32 => sk0{1}.[4 + k] = nth witness sk_seed{2} k) /\
-  (forall (k : int), 0 <= k < 32 => sk0{1}.[4 + 32 + k] = nth witness sk_prf{2} k) /\
-  (forall (k : int), 0 <= k < 32 => sk0{1}.[4 + 3 * 32 + k] = nth witness pub_seed{2} k)
+  (forall (k : int), 0 <= k < 32 => sk0{1}.[4 + k] = nth witness (val sk_seed{2}) k) /\
+  (forall (k : int), 0 <= k < 32 => sk0{1}.[4 + 32 + k] = nth witness (val sk_prf{2}) k) /\
+  (forall (k : int), 0 <= k < 32 => sk0{1}.[4 + 3 * 32 + k] = nth witness (val pub_seed{2}) k)
 ).
-    + auto => /> &1 &2 H0 H1 H2 H3 H4 H5 H6 H7 H8 H9 H10 H11; do split => k??; rewrite initiE 1:/#; auto => />; first by smt(). 
-       * rewrite ifF 1:/# -H9 //=.  
-       * rewrite ifF 1:/# -H10 //=.
-       * rewrite ifT 1:/# -H6 //= H11 //=. 
-
-(* At this point, sk has all the fields set (except for the root) *)
-
+    + auto => /> &1 &2 H0 H1 H2 H3 H4 H5 H6 H7 H8. 
+      do split => k??; rewrite initiE 1:/#; auto => />; first by smt().
+       * by rewrite ifF 1:/# H6.  
+       * by rewrite ifF 1:/# -H7.
+       * by rewrite ifT 1:/# -H3 //= H8. 
 seq 2 0 : (
   #pre /\
   (forall (k : int), 0 <= k < 32 => bufn1{1}.[k] = sk0{1}.[100 + k]) 
 ); first by auto => /> *; rewrite initiE /#. 
 seq 1 0 : (#pre /\ bufn0{1} = bufn1{1}); first by ecall {1} (_x_memcpy_u8u8_post bufn1{1}); skip => />. 
-
 seq 1 0 : (
-  to_list seed_p{1} = sk_seed{2} ++ sk_prf{2} ++ pub_seed{2} /\
-  size sk_seed{2} = 32 /\
-  size sk_prf{2} = 32 /\
-  size pub_seed{2} = 32 /\
+  to_list seed_p{1} = val sk_seed{2} ++ val sk_prf{2} ++ val pub_seed{2} /\
   seed0{1} = seed_p{1} /\
   address{2} = top_tree_addr{1} /\
 
-  (forall (k : int), 0 <= k < 32 => seed_p{1}.[k] = nth witness sk_seed{2} k) /\
-  (forall (k : int), 0 <= k < 32 => seed_p{1}.[32 + k] = nth witness sk_prf{2} k) /\
-  (forall (k : int), 0 <= k < 32 => seed_p{1}.[64 + k] = nth witness pub_seed{2} k) /\
+  (forall (k : int), 0 <= k < 32 => seed_p{1}.[k] = nth witness (val sk_seed{2}) k) /\
+  (forall (k : int), 0 <= k < 32 => seed_p{1}.[32 + k] = nth witness (val sk_prf{2}) k) /\
+  (forall (k : int), 0 <= k < 32 => seed_p{1}.[64 + k] = nth witness (val pub_seed{2}) k) /\
 
   to_list idx{1} = nseq 4 W8.zero /\
 
 
   (forall (k : int), 0 <= k < 4 => sk0{1}.[k] = W8.zero) /\
-  (forall (k : int), 0 <= k < 32 => sk0{1}.[4 + k] = nth witness sk_seed{2} k) /\
-  (forall (k : int), 0 <= k < 32 => sk0{1}.[4 + 32 + k] = nth witness sk_prf{2} k) /\
-  (forall (k : int), 0 <= k < 32 => sk0{1}.[4 + 3 * 32 + k] = nth witness pub_seed{2} k) /\
+  (forall (k : int), 0 <= k < 32 => sk0{1}.[4 + k] = nth witness (val sk_seed{2}) k) /\
+  (forall (k : int), 0 <= k < 32 => sk0{1}.[4 + 32 + k] = nth witness (val sk_prf{2}) k) /\
+  (forall (k : int), 0 <= k < 32 => sk0{1}.[4 + 3 * 32 + k] = nth witness (val pub_seed{2}) k) /\
 
-  (forall (k : int), 0 <= k < 32 => pk0{1}.[32 + k] = nth witness pub_seed{2} k) (* this is the pub seed *)
+  (forall (k : int), 0 <= k < 32 => pk0{1}.[32 + k] = nth witness (val pub_seed{2}) k) (* this is the pub seed *)
 ).
-    + auto => /> &1 &2 H0 H1 H2 H3 H4 H5 H6 H7 H8 H9 H10 H11 H12 k ??.
-      rewrite initE ifT 1:/#; auto => />.
-      rewrite ifT 1:/# -H11 1:/# H12 //=.  
-
+    + auto => /> &1 &2 H0 H1 H2 H3 H4 H5 H6 H7 H8 H9 k??.
+      rewrite initE ifT 1:/# => />.
+      by rewrite ifT 1:/# -H8 1:/# H9.  
 seq 2 0 : (
   #pre /\
-  to_list bufn0{1} = sk_seed{2} /\
-  to_list bufn1{1} = pub_seed{2}
+  to_list bufn0{1} = val sk_seed{2} /\
+  to_list bufn1{1} = val pub_seed{2}
 ).
-    + auto => /> &1 &2 H0 H1 H2 H3 H4 H5 H6 H7 H8 H9 H10 H11 H12; split. 
-        - apply (eq_from_nth witness); [by rewrite size_to_list H1 | rewrite size_to_list => i?].
-          rewrite get_to_list initiE 1:/#; auto => />; rewrite -H9 //=.
-        - apply (eq_from_nth witness); [by rewrite size_to_list H3 | rewrite size_to_list => i?].
-          rewrite get_to_list initiE 1:/#; auto => />; rewrite H12 1:/# //=.
-
+    + auto => /> &1 &2 H0 H1 H2 H3 H4 H5 H6 H7 H8 H9; split.
+        - apply (eq_from_nth witness); [by rewrite valP size_to_list n_val |].
+          rewrite size_to_list => i?.
+          rewrite get_to_list initiE 1:/# => />. 
+          by rewrite -H6.
+        - apply (eq_from_nth witness); [by rewrite valP size_to_list n_val |].
+          rewrite size_to_list => i?.
+          rewrite get_to_list initiE 1:/# => />. 
+          by apply H9.
 seq 0 1 : (
     #pre /\ 
-    toByte sk{2}.`idx 4 = sub sk0{1} 0  4  /\
-    sk{2}.`sk_seed      = sub sk0{1} 4  32 /\
-    sk{2}.`sk_prf       = sub sk0{1} 36 32 /\
-    sk{2}.`pub_seed_sk  = sub sk0{1} 100 32 (* NOTA: a pub seed e a root estao trocadas => Na spec a root vem no fim mas na impl no fim esta a pub seed => a root esta entre a sk prf e a pub seed *)
+    toByte sk{2}.`idx 4     = sub sk0{1} 0  4  /\ 
+    val sk{2}.`sk_seed      = sub sk0{1} 4  32 /\
+    val sk{2}.`sk_prf       = sub sk0{1} 36 32 /\
+    val sk{2}.`pub_seed_sk  = sub sk0{1} 100 32 
+    (* NOTA: a pub seed e a root estao trocadas => Na spec a root vem no fim mas na impl no fim esta a pub seed => a root esta entre a sk prf e a pub seed *)
 ).
 
-    + auto => /> &1 &2 H0 H1 H2 H3 H4 H5 H6 H7 H8 H9 H10 H11 H12; do split.
+    + auto => /> &1 &2 H0 H1 H2 H3 H4 H5 H6 H7 H8 H9 H10 H11; do split.
       * apply (eq_from_nth witness); rewrite /toByte size_take //= size_rev size_to_list //=; [ by rewrite size_sub //= |] => i?. 
         rewrite nth_sub //= nth_take //= 1:/# nth_rev 1:#smt:(size_to_list) size_to_list //=.
         have ->: to_list (unpack8 W32.zero) = nseq 4 W8.zero.
              - apply (eq_from_nth W8.zero); [ by rewrite size_to_list size_nseq |].
                rewrite size_to_list => j?.
                rewrite get_to_list nth_nseq //= get_unpack8 //= get_zero //.
-        rewrite nth_nseq 1:/# H8 //=.    
-      * apply (eq_from_nth witness); [by rewrite size_to_list size_sub | rewrite size_to_list] => i?.
-        rewrite get_to_list nth_sub //= H9 //.
-      * apply (eq_from_nth witness); [by rewrite H2 size_sub | rewrite H2] => i?.
-        rewrite nth_sub //= H10 //.
-      * apply (eq_from_nth witness); [by rewrite size_to_list size_sub | rewrite size_to_list] => i?.
-        rewrite nth_sub //= -H11 //=.
-
-seq 1 1 : (#pre /\ root{2} = to_list root{1}).
+        by rewrite nth_nseq 1:/# H5.  
+      * apply (eq_from_nth witness); [by rewrite size_sub // valP n_val |]. 
+        rewrite valP n_val => ??.
+        by rewrite -H6 // nth_sub.
+      * apply (eq_from_nth witness); [by rewrite size_sub // valP n_val |]. 
+        rewrite valP n_val => ??.
+        by rewrite -H7 // nth_sub.
+      * apply (eq_from_nth witness); [by rewrite size_sub // valP n_val |]. 
+        rewrite valP n_val => ??.
+        by rewrite -H8 // nth_sub.
+seq 1 1 : (#pre /\ val root{2} = to_list root{1}).
     + admit. (* call to treehash lemma *)
 
 seq 1 0  : ( 
   #pre /\
-  (forall (k : int), 0 <= k < 32 => pk0{1}.[k] = nth witness root{2} k)
+  (forall (k : int), 0 <= k < 32 => pk0{1}.[k] = nth witness (val root{2}) k)
 ).
-    + inline {1}. wp.
+    + inline {1}. 
+      wp.
       while {1}  
       (
         #pre /\  
@@ -314,17 +283,22 @@ seq 1 0  : (
       (32 - i{1}); last first. (* FIXME: TODO: Remover lemmas de pk0 da #pre *)
         - auto => /> &1 &2 H0 H1 H2 H3 H4 H5 H6 H7 H8 H9 H10 H11 H12 H13 H14 H15 H16 *; split => [/# | iL];  split => [/# | ???]. 
           have ->: iL = 32 by smt(). 
-          move => H17 /#. 
-        - auto => /> &hr *; do split; 1,2,5:smt(). 
-             * rewrite tP => *; admit.
+          move => H17 k??.
+          rewrite H16 get_to_list /#.
+        - auto => /> &hr *; do split; 1,2,5:smt().  
+             * rewrite tP => j?.
+               rewrite get_setE; first by rewrite of_uintK /#.  
+               rewrite of_uintK (: i{hr} %% W64.modulus  = i{hr}) 1:/#. 
+               case (j = i{hr}) => ? //.
+               admit.
              * move => k??; rewrite get_setE; [by split; by rewrite of_uintK /# |]. 
                rewrite of_uintK (: i{hr} %% W64.modulus = i{hr}) /#.  
-
 seq 1 0 : (
   #pre /\
-  (forall (k : int), 0 <= k < 32 => sk0{1}.[4 + 2 * 32 + k] = nth witness root{2} k)
-). 
-    + inline {1}.  wp.
+  (forall (k : int), 0 <= k < 32 => sk0{1}.[4 + 2 * 32 + k] = nth witness (val root{2}) k)
+).
+    + inline {1}.  
+      wp.
       while {1} 
       (
         #pre /\ 
@@ -335,45 +309,61 @@ seq 1 0 : (
         in_0{1} = root{1} /\
         (forall (k : int), 0 <= k < i{1} => out{1}.[4 + 2 * 32 + k] = in_0{1}.[k])
       ) 
-      (32 - i{1}); last by auto => /> /#.
-      auto => /> &hr *. do split;1,2,5:smt(). 
-          * admit. 
-          * move => k??. rewrite get_setE 1:#smt:(@W64 pow2_64). 
-            case (68 + k = to_uint (offset_out{hr} + (of_int i{hr})%W64)) => ?. admit. admit. 
+      (32 - i{1}); last first.
+          * auto => /> &1 &2 H0 H1 H2 H3 H4 H5 H6 H7 H8 H9 H10 H11 H12 H13 H14 H15 H16 H17. 
+            do 2! (split => [/# | *]). 
+            rewrite H16 get_to_list /#. 
+      auto => /> &hr H0 H1 H2 H3 H4 H5 H6 H7 H8 H9 H10 H11 H12 H13 H14 H15 H16 H17 H18 H19 H20 H21 H22 *. 
+      do split;1,2,5:smt(). 
+          * rewrite tP => j?.  
+            rewrite get_setE 1:#smt:(@W64 pow2_64).
+            case (j = to_uint (offset_out{hr} + (of_int i{hr})%W64)) => ? //.
+            rewrite of_uintK (: i{hr} %% W64.modulus = i{hr}) 1:/#. 
+            admit.
+          * move => k??.
+            rewrite get_setE 1:#smt:(@W64 pow2_64). 
+            case (68 + k = to_uint (offset_out{hr} + (of_int i{hr})%W64)) => ?. 
+                - admit.
+                - admit.
+
 auto => /> &1 &2 H0 H1 H2 H3 H4 H5 H6 H7 H8 H9 H10 H11 H12 H13 H14 H15 H16 H17 H18; split.
     + rewrite /DecodePkNoOID => />; rewrite tP => i Hi.
       rewrite get_of_list //=.
       case (0 <= i < 32).
         + move => ?.
-          rewrite nth_cat size_to_list ifT 1:/# get_to_list H17 //=.
+          by rewrite nth_cat valP n_val ifT 1:/#  H17.  
         + move => ?. 
-          rewrite nth_cat size_to_list ifF 1:/# get_to_list -H12 //= /#.
-    + rewrite /DecodeSkNoOID => />; rewrite tP => i Hi. rewrite -!get_to_list.
+          rewrite nth_cat valP n_val ifF 1:/#.
+          admit.
+    + rewrite /DecodeSkNoOID => />; rewrite tP => i Hi. 
+      rewrite -!get_to_list.
       case (0 <= i < 4).
         + move => ?. 
-          rewrite of_listK; [by rewrite !size_cat !size_to_list H2 size_W32toBytes |].
-          do ! (rewrite nth_cat !size_cat !size_to_list H2 size_W32toBytes //= ifT 1:/#).
-          rewrite nth_cat !size_cat !size_to_list size_W32toBytes //= ifT 1:/#.
-          rewrite nth_cat size_W32toBytes ifT 1:/# W32toBytes_zero_nth //= H8 //=.
+          rewrite of_listK; first by rewrite !size_cat !valP n_val size_W32toBytes.
+          do 3! (rewrite nth_cat !size_cat !valP n_val size_W32toBytes /= ifT 1:/#).
+          rewrite nth_cat size_W32toBytes //= ifT 1:/# W32toBytes_zero_nth //=.
+          by apply H5.
       case (4 <= i < 4 + 32).
         + simplify => ? _. 
           rewrite get_of_list //=.
-          rewrite nth_cat !size_cat !size_to_list size_W32toBytes H2 //= ifT 1:/#.
-          rewrite nth_cat !size_cat !size_to_list size_W32toBytes H2 //= ifT 1:/#.
-          rewrite nth_cat !size_cat !size_to_list size_W32toBytes //= ifT 1:/#.  
-          rewrite nth_cat size_W32toBytes //= ifF 1:/# -H9 //= /#.  
+          do 3! (rewrite nth_cat !size_cat size_W32toBytes !valP n_val /= ifT 1:/#).
+          rewrite nth_cat size_W32toBytes //= ifF 1:/#. 
+          rewrite -H6 // /#. 
       case (4 + 32 <= i < 4 + 2 * 32).
         + simplify => ? _ _.
           rewrite get_of_list //=.
-          rewrite nth_cat !size_cat !size_to_list size_W32toBytes H2 //= ifT 1:/#.
-          rewrite nth_cat !size_cat !size_to_list size_W32toBytes H2 //= ifT 1:/#.
-          rewrite nth_cat !size_cat !size_to_list size_W32toBytes //= ifF 1:/# -H10 //= /#.  
+          rewrite nth_cat !size_cat size_W32toBytes !valP n_val /= ifT 1:/#.
+          rewrite nth_cat !size_cat size_W32toBytes !valP n_val /= ifT 1:/#.
+          rewrite nth_cat !size_cat size_W32toBytes !valP n_val /= ifF 1:/#.
+          rewrite -H7 /#.
       case (4 + 2*32 <= i < 4 + 3*32).     
         + simplify => ? _ _ _.
           rewrite get_of_list //=.
-          rewrite nth_cat !size_cat !size_to_list size_W32toBytes H2 //= ifT 1:/#.
-          rewrite nth_cat !size_cat !size_to_list size_W32toBytes H2 //= ifF 1:/# -H18 /#.
+          rewrite nth_cat !size_cat size_W32toBytes !valP n_val /= ifT 1:/#.
+          rewrite nth_cat !size_cat size_W32toBytes !valP n_val /= ifF 1:/#.
+          rewrite -H18 /#.
       move => ????.      
-      rewrite get_to_list of_listK; [by rewrite !size_cat !size_to_list size_W32toBytes H2|].
-      rewrite nth_cat !size_cat !size_to_list size_W32toBytes H2 //= ifF 1:/# -H11 /#.
+      rewrite get_to_list of_listK; [by rewrite !size_cat !valP n_val size_W32toBytes |].
+     rewrite nth_cat !size_cat !valP n_val size_W32toBytes /= ifF /#.
 qed.
+
